Binary Subtraction

IMP--_To_SAS+/IMP_Minus_To_IMP_Minus_Minus_State_Translations.thy
@@ -5,6 +5,102 @@ section "IMP- to IMP-- State Translations"
 theory IMP_Minus_To_IMP_Minus_Minus_State_Translations imports "../IMP-/Small_StepT" IMP_Minus_Minus_Small_StepT 
 begin 
 
+definition var_to_var_bit:: "vname \<Rightarrow> (vname * nat) option" where
+"var_to_var_bit v = (if length v > 0 then (if hd v = CHR ''#'' 
+  then (let t = dropWhile (\<lambda>i. i = CHR ''#'') v; 
+  l = length (takeWhile (\<lambda>i. i = CHR ''#'') v) - 1 in
+  (if length t > 0 \<and> hd t = CHR ''$'' then Some (tl t, l) else None))
+  else None)
+  else None)"
 
+fun n_hashes:: "nat \<Rightarrow> string" where
+"n_hashes 0 = []" |
+"n_hashes (Suc n) = (CHR ''#'') # (n_hashes n)" 
+
+definition var_bit_to_var:: "(vname * nat) \<Rightarrow> vname" where
+"var_bit_to_var vk = (n_hashes (snd vk + 1)) @ ''$''  @ (fst vk)" 
+
+lemma dropWhile_n_hashes[simp]: "dropWhile (\<lambda>i. i = CHR ''#'') (n_hashes x @ CHR ''$'' # y) 
+  = CHR ''$'' # y" 
+  apply(induction x)
+  by(auto)
+
+lemma length_takeWhile_n_hashes[simp]: 
+  "length (takeWhile (\<lambda>i. i = CHR ''#'') (n_hashes x @ CHR ''$'' # y)) = x"
+  apply(induction x)
+  by auto
+
+lemma encoded_var_decomposition[simp]: "x \<noteq> [] \<Longrightarrow> hd x = CHR ''#''
+  \<Longrightarrow> hd (dropWhile (\<lambda>i. i = CHR ''#'') x) = CHR ''$'' 
+  \<Longrightarrow> c \<in> set x \<Longrightarrow> c \<noteq> CHR ''#''
+  \<Longrightarrow> n_hashes (length (takeWhile (\<lambda>i. i = CHR ''#'') x)) 
+    @ CHR ''$'' # tl (dropWhile (\<lambda>i. i = CHR ''#'') x) = x"
+proof (induction x)
+  case (Cons a x)
+  hence *: "x \<noteq> []" by auto
+  have "hd x = CHR ''#'' \<or> hd x \<noteq> CHR ''#''" by auto
+  thus ?case
+    apply(elim disjE)
+    using Cons * apply(auto)
+    by (smt hd_Cons_tl list.size(3) n_hashes.simps(1) self_append_conv2 takeWhile.simps(1) 
+        takeWhile_dropWhile_id takeWhile_tail)
+qed auto
+
+lemma var_to_var_bit_var_bit_to_var[simp]: "var_to_var_bit (var_bit_to_var x) = Some x" 
+  by (auto simp: var_to_var_bit_def var_bit_to_var_def Let_def)
+
+lemma var_to_var_bit_eq_Some_iff: "var_to_var_bit x = Some y \<longleftrightarrow> x = var_bit_to_var y" 
+proof
+  assume "var_to_var_bit x = Some y" 
+  thus "x = var_bit_to_var y" 
+    apply(auto simp: var_to_var_bit_def var_bit_to_var_def Let_def split: if_splits)
+    using encoded_var_decomposition 
+    by (smt Nitpick.size_list_simp(2) One_nat_def char.inject length_tl list.expand list.sel(1) 
+        list.sel(3) list.simps(3) n_hashes.simps(2) self_append_conv2 
+        takeWhile_dropWhile_id tl_append2)
+qed auto
+
+lemma var_bit_to_var_eq_iff: "var_bit_to_var (a, b) = var_bit_to_var (c, d) \<longleftrightarrow> (a = c \<and> b = d)" 
+  apply(auto simp: var_bit_to_var_def)
+   apply (metis dropWhile_n_hashes list.inject)
+  by (metis length_takeWhile_n_hashes)
+
+lemma var_to_var_bit_of_non_zero_indicator[simp]: "var_to_var_bit (CHR ''?'' # CHR ''$'' # v) = None" 
+  by(auto simp: var_to_var_bit_def)
+
+lemma var_bit_to_var_neq_non_zero_indicator[simp]: "(''?$'' @ x \<noteq> var_bit_to_var (v, y))"
+  by(auto simp: var_bit_to_var_def)
+
+lemma var_bit_to_var_neq_non_zero_indicator'[simp]: "(var_bit_to_var (a, b) = CHR ''?'' # CHR ''$'' # v) 
+  \<longleftrightarrow> False"
+  by(auto simp: var_bit_to_var_def)
+
+lemma var_to_var_bit_of_carry[simp]: "var_to_var_bit ''carry'' = None"
+  by(auto simp: var_to_var_bit_def)
+
+lemma var_bit_to_var_neq_carry[simp]: "''carry'' \<noteq> var_bit_to_var (x, y) "
+  by(auto simp: var_bit_to_var_def)
+
+lemma var_bit_to_var_neq_carry'[simp]: "var_bit_to_var (x, y) = ''carry'' \<longleftrightarrow> False"
+  by(auto simp: var_bit_to_var_def)
+
+fun nth_bit:: "nat \<Rightarrow> nat \<Rightarrow> nat" where
+"nth_bit x 0 = x mod 2" |
+"nth_bit x (Suc n) = nth_bit (x div 2) n"
+
+lemma zero_le_nth_bit_then[simp]: "0 < nth_bit x n \<longleftrightarrow> nth_bit x n = 1" 
+  apply(induction n arbitrary: x)
+  by auto
+
+lemma nth_bit_of_zero[simp]: "nth_bit 0 n = 0" 
+  by (induction n) auto
+
+lemma nth_bit_eq_zero_or_one: "nth_bit x n = y \<Longrightarrow> (y = 0 \<or> y = 1)" 
+  by (induction n arbitrary: x) auto
+
+definition IMP_Minus_State_To_IMP_Minus_Minus:: "state \<Rightarrow> nat \<Rightarrow> state" where
+"IMP_Minus_State_To_IMP_Minus_Minus s n = (\<lambda>v. (case var_to_var_bit v of 
+  Some (v', k) \<Rightarrow> if k < n then nth_bit (s v') k else 0 |
+  None \<Rightarrow> (if length v > 1 \<and> take 2 v = ''?$'' \<and> (s (tl v)) > 0 then 1 else 0)))"
 
 end
