IMP--_To_SAS+/Binary_Operations.thy
@@ -1,0 +1,603 @@
+\<^marker>\<open>creator Florian Keßler\<close>
+
+section "Binary Operations in IMP--"
+
+theory Binary_Operations imports IMP_Minus_To_IMP_Minus_Minus_State_Translations
+begin 
+
+type_synonym IMP_Minus_com = Com.com
+type_synonym IMP_Minus_Minus_com = com
+
+unbundle Com.no_com_syntax
+
+fun com_list_to_seq:: "IMP_Minus_Minus_com list \<Rightarrow> IMP_Minus_Minus_com" where
+"com_list_to_seq [] = SKIP" | 
+"com_list_to_seq (c # cs) = c ;; (com_list_to_seq cs)"
+
+lemma t_small_step_fun_com_list_to_seq_terminates: "t1 + t2 < t
+  \<Longrightarrow> t_small_step_fun t1 (com_list_to_seq as, s1) = (SKIP, s3)
+  \<Longrightarrow> t_small_step_fun t2 (com_list_to_seq bs, s3) = (SKIP, s2)
+  \<Longrightarrow> t_small_step_fun t (com_list_to_seq (as @ bs), s1) = (SKIP, s2)"
+proof(induction as arbitrary: s1 t1 t)
+  case Nil
+  then show ?case using t_small_step_fun_increase_time 
+    by (metis Pair_inject append_self_conv2 com_list_to_seq.simps le_add2 
+        less_imp_le_nat t_small_step_fun_SKIP)
+next
+  case (Cons a as)
+  then obtain ta sa where ta_def: "ta < t1 \<and> t_small_step_fun ta (a, s1) = (SKIP, sa) 
+    \<and> t_small_step_fun (t1 - (ta + 1)) (com_list_to_seq as, sa) = (SKIP, s3)"
+    by (auto simp: seq_terminates_iff)
+  hence "t_small_step_fun (t - (ta + 1)) (com_list_to_seq (as @ bs), sa) = (SKIP, s2)"  
+    apply -
+    apply(rule Cons(1))
+    using Cons by(auto)
+  thus ?case using ta_def Cons seq_terminates_iff by fastforce
+qed
+
+fun binary_assign_constant:: "nat \<Rightarrow> vname \<Rightarrow> nat \<Rightarrow> IMP_Minus_Minus_com" where 
+"binary_assign_constant 0 v x = SKIP" |
+"binary_assign_constant (Suc n) v x = (var_bit_to_var (v, n)) ::= A (N (nth_bit x n)) ;;
+  binary_assign_constant n v x" 
+
+lemma result_of_binary_assign_constant: "t_small_step_fun (3 * n) 
+  (binary_assign_constant n v x, s) 
+  = (SKIP, \<lambda>w. (case var_to_var_bit w of
+      Some (w', m) \<Rightarrow> (if w' = v \<and> m < n then nth_bit x m else s w) |
+      _ \<Rightarrow> s w))"
+proof(induction n arbitrary: s)
+  case (Suc n)
+  thus ?case 
+    apply auto
+    apply(rule seq_terminates_when[where ?t1.0=1 and ?t2.0="3*n" and 
+          ?s3.0="s(var_bit_to_var (v, n) := nth_bit x n)"])
+    by(auto simp: fun_eq_iff var_to_var_bit_eq_Some_iff var_bit_to_var_eq_iff split: option.splits)
+qed (auto simp: fun_eq_iff split: option.splits)
+
+fun nth_carry:: "nat \<Rightarrow> nat \<Rightarrow> nat \<Rightarrow> nat" where
+"nth_carry 0 a b = (if (nth_bit a 0 = 1 \<and> nth_bit b 0 = 1) then 1 else 0)" | 
+"nth_carry (Suc n) a b = (if (nth_bit a (Suc n) = 1 \<and> nth_bit b (Suc n) = 1) 
+  \<or> ((nth_bit a (Suc n) = 1 \<or> nth_bit b (Suc n) = 1) \<and> nth_carry n a b = 1) then 1 else 0)"
+
+lemma zero_le_nth_carry_then[simp]: "0 < nth_carry n a b \<longleftrightarrow> nth_carry n a b = 1" 
+  apply(cases n)
+  by(auto split: if_splits)
+
+lemma first_bit_of_add: "nth_bit (a + b) 0 = (if nth_bit a 0 + nth_bit b 0 = 1 then 1 else 0)" 
+  apply(induction a)
+   apply(auto split: if_splits)
+  by presburger+
+
+lemma nth_bit_of_add: "nth_bit (a + b) (Suc n) = (let s = nth_bit a (Suc n) + nth_bit b (Suc n) 
+  + nth_carry n a b in (if s = 1 \<or> s = 3 then 1 else 0))" 
+  sorry
+
+lemma no_overflow_condition: "a + b < 2^n \<Longrightarrow> nth_carry (n - 1) a b = 0" 
+  sorry
+
+lemma all_bits_in_sum_zero_then: "(\<forall>i \<le> k. nth_bit (a + b) i = 0) 
+  \<Longrightarrow> (a + b \<ge> 2^(k + 1) \<or> (a = 0 \<and> b = 0))"
+  sorry
+
+lemma has_bit_one_then_greater_zero: "nth_bit a j = Suc 0 \<Longrightarrow> 0 < a" 
+  sorry
+
+fun nth_carry_sub:: "nat \<Rightarrow> nat \<Rightarrow> nat \<Rightarrow> nat" where
+"nth_carry_sub 0 a b = (if (nth_bit a 0 = 0 \<and> nth_bit b 0 = 1) then 1 else 0)" | 
+"nth_carry_sub (Suc n) a b = (if nth_bit a (Suc n) < nth_bit b (Suc n) + nth_carry_sub n a b then 1
+  else 0)"
+
+lemma nth_carry_sub_leq_one: "nth_carry_sub n a b = x \<Longrightarrow> (x = 0 \<or> x = 1)"
+  by (metis nth_carry_sub.elims)
+
+lemma nth_carry_sub__neq_one_iff[simp]: "nth_carry_sub n a b \<noteq> Suc 0 \<longleftrightarrow> nth_carry_sub n a b = 0" 
+  using nth_carry_sub_leq_one by auto
+
+lemma nth_bit_of_sub_n_no_underflow: "a \<ge> b \<Longrightarrow> 
+  nth_bit (a - b) (Suc n) = (let an = nth_bit a (Suc n); bn = nth_bit b (Suc n);
+  c = nth_carry_sub n a b in (if  bn + c = 0 \<or> bn + c = 2 then an 
+    else (if bn + c = 1 \<and> an = 0 then 1 else 0)))" 
+  sorry
+
+lemma nth_bit_of_sub_n_underflow: "a < b \<Longrightarrow> 
+  nth_bit (a - b) (Suc n) = 0" 
+  by simp
+
+fun operand_bit_to_var:: "(char * nat) \<Rightarrow> vname" where 
+"operand_bit_to_var (c, 0) = [c]" |
+"operand_bit_to_var (c, (Suc n)) = c # operand_bit_to_var (c, n)"
+
+definition var_to_operand_bit:: "vname \<Rightarrow> (char * nat) option" where
+"var_to_operand_bit v = (if v \<noteq> [] \<and> v = (operand_bit_to_var (hd v, length v - 1)) 
+  then Some (hd v, length v - 1) else None)" 
+
+lemma hd_of_operand_bit_to_var[simp]: 
+  "hd (operand_bit_to_var (op, n)) = op" by (induction n) auto
+
+lemma length_of_operand_bit_to_var[simp]:
+  "length (operand_bit_to_var (op, n)) = n + 1" by (induction n) auto  
+
+lemma var_to_operand_bit_of_operand_bit_to_var[simp]: 
+  "var_to_operand_bit (operand_bit_to_var (op, n)) = Some (op, n)"
+  apply(induction n)
+  by(auto simp: var_to_operand_bit_def)
+
+lemma var_to_operand_bit_eq_Some_iff: "var_to_operand_bit x = Some (op, i) 
+  \<longleftrightarrow> x = operand_bit_to_var (op, i)" 
+  apply(auto simp: var_to_operand_bit_def)
+  apply(cases i)
+  by auto
+
+lemma var_to_operand_bit_of_carry[simp]: "var_to_operand_bit ''carry'' = None" 
+  by(simp add: var_to_operand_bit_def)
+
+lemma set_of_operand_bit_to_var[simp]: "set (operand_bit_to_var (op, b)) = { op }" 
+  by (induction b) auto
+
+lemma var_to_operand_bit_var_bit_to_var[simp]: "var_to_operand_bit (var_bit_to_var (a, b)) = None" 
+  apply(simp add: var_to_operand_bit_def var_bit_to_var_def)
+  apply(rule ccontr)
+  apply simp
+  apply(drule arg_cong[where ?f=set])
+  by simp
+
+lemma var_to_var_bit_operand_bit_to_var[simp]: "var_to_var_bit (operand_bit_to_var (c, k)) = None" 
+  by (simp add: var_to_var_bit_def)
+
+lemma var_to_operand_bit_non_zero_indicator[simp]: 
+  "var_to_operand_bit (CHR ''?'' # CHR ''$'' # v) = None"
+  apply(auto simp: var_to_operand_bit_def)
+  apply(rule ccontr)
+  apply simp
+  apply(drule arg_cong[where ?f=set])
+  by simp
+
+lemma operand_bit_to_var_ne_non_zero_indicator[simp]: 
+  "operand_bit_to_var (c, k) \<noteq> CHR ''?'' # CHR ''$'' # v" 
+  apply(induction k)
+   apply auto
+proof -
+  fix ka :: nat
+  assume "operand_bit_to_var (CHR ''?'', ka) = CHR ''$'' # v"
+  then have "CHR ''?'' = CHR ''$''" by (metis hd_of_operand_bit_to_var list.sel(1))
+  then show False by force
+qed
+
+lemma operand_bit_to_var_non_empty: "operand_bit_to_var (op, n) \<noteq> []"
+  by (induction n) auto
+
+lemma operand_bit_to_var_eq_operand_bit_to_var_iff[simp]: 
+  "operand_bit_to_var (op, a) = operand_bit_to_var (op', b) 
+  \<longleftrightarrow> (op = op' \<and> a = b)" 
+proof 
+  assume "operand_bit_to_var (op, a) = operand_bit_to_var (op', b)" 
+  hence "length (operand_bit_to_var (op, a)) = length (operand_bit_to_var (op', b))
+    \<and> set (operand_bit_to_var (op, a)) = set (operand_bit_to_var (op', b))" by simp
+  thus "op = op' \<and> a = b" by auto
+qed auto
+
+lemma var_bit_to_var_neq_operand_bit_to_var[simp]: 
+  "var_bit_to_var (v, a) \<noteq> operand_bit_to_var (op, b)"
+proof(rule ccontr)
+  assume "\<not> (var_bit_to_var (v, a) \<noteq> operand_bit_to_var (op, b))" 
+  hence "set (var_bit_to_var (v, a)) = set (operand_bit_to_var (op, b))" by simp
+  thus False using set_of_operand_bit_to_var by(auto simp: var_bit_to_var_def)
+qed
+
+fun copy_var_to_operand:: "nat \<Rightarrow> char \<Rightarrow> vname \<Rightarrow> IMP_Minus_Minus_com" where
+"copy_var_to_operand 0 op v = SKIP" |
+"copy_var_to_operand (Suc i) op v = 
+   (operand_bit_to_var (op, i)) ::= A (V (var_bit_to_var (v, i))) ;;
+    copy_var_to_operand i op v " 
+
+lemma copy_var_to_operand_result:
+  "t_small_step_fun (2 * n) (copy_var_to_operand n op v, s)
+  = (SKIP, \<lambda>w. (case var_to_operand_bit w of
+    Some (op', i) \<Rightarrow> (if op' = op \<and> i < n then s (var_bit_to_var (v, i)) else s w) |
+    _ \<Rightarrow> s w))" 
+  apply(induction n arbitrary: s)
+   apply(auto simp: fun_eq_iff var_to_operand_bit_eq_Some_iff split!: option.splits if_splits)
+  using less_antisym by blast
+
+fun copy_const_to_operand:: "nat \<Rightarrow> char \<Rightarrow> nat \<Rightarrow> IMP_Minus_Minus_com" where
+"copy_const_to_operand 0 op x = SKIP" |
+"copy_const_to_operand (Suc i) op x = 
+   (operand_bit_to_var (op, i)) ::= A (N (nth_bit x i)) ;;
+    copy_const_to_operand i op x " 
+
+lemma copy_const_to_operand_result:
+  "t_small_step_fun (2 * n) (copy_const_to_operand n op x, s)
+  = (SKIP, \<lambda>w. (case var_to_operand_bit w of
+    Some (op', i) \<Rightarrow> (if op' = op \<and> i < n then nth_bit x i else s w) |
+    _ \<Rightarrow> s w))" 
+  apply(induction n arbitrary: s)
+   apply(auto simp: fun_eq_iff var_to_operand_bit_eq_Some_iff split!: option.splits if_splits)
+  using less_antisym by blast
+
+definition assign_var_carry:: 
+  "nat \<Rightarrow> vname \<Rightarrow> nat \<Rightarrow> nat \<Rightarrow> nat \<Rightarrow> IMP_Minus_Minus_com" where
+"assign_var_carry i v a b c = 
+  (var_bit_to_var (v, i)) ::= A (N (if a + b + c = 1 \<or> a + b + c = 3 then 1 else 0)) ;; 
+  ''carry'' ::= A (N (if a + b + c \<ge> 2 then 1 else 0))"
+
+lemma result_of_assign_var_carry:  
+  "t_small_step_fun 7 (assign_var_carry i v a b c, s)
+    = (SKIP, s(var_bit_to_var (v, i) := (if a + b + c = 1 \<or> a + b + c = 3 then 1 else 0),
+     ''carry'' :=  (if a + b + c \<ge> 2 then 1 else 0)))"
+  by(auto simp: assign_var_carry_def t_small_step_fun_terminate_iff)
+
+definition full_adder:: "nat \<Rightarrow> vname \<Rightarrow> IMP_Minus_Minus_com" where
+"full_adder i v  = (let assign = assign_var_carry i v; op_a = operand_bit_to_var (CHR ''a'', i);
+  op_b = operand_bit_to_var (CHR ''b'', i) in 
+  IF op_a\<noteq>0 THEN 
+    IF ''carry''\<noteq>0 THEN
+      IF op_b\<noteq>0 THEN assign 1 1 1 
+      ELSE assign 1 1 0
+    ELSE 
+      IF op_b\<noteq>0 THEN assign 1 0 1
+      ELSE assign 1 0 0
+  ELSE 
+    IF ''carry''\<noteq>0 THEN
+      IF op_b\<noteq>0 THEN assign 0 1 1
+      ELSE assign 0 1 0
+    ELSE 
+      IF op_b\<noteq>0 THEN assign 0 0 1
+      ELSE assign 0 0 0)"
+
+lemma full_adder_correct: 
+  assumes "i = 0 \<longrightarrow> s ''carry'' = 0" 
+    "i > 0 \<longrightarrow> s ''carry'' = nth_carry (i - 1) a b"
+    "s (operand_bit_to_var (CHR ''a'', i)) = nth_bit a i" 
+    "s (operand_bit_to_var (CHR ''b'', i)) = nth_bit b i"
+  shows "t_small_step_fun 10 (full_adder i v, s) = (SKIP, 
+    s(var_bit_to_var (v, i) := nth_bit (a + b) i, ''carry'' := nth_carry i a b))" 
+  using assms 
+  apply(simp add: full_adder_def Let_def t_small_step_fun_terminate_iff result_of_assign_var_carry)
+  apply(cases i)
+  apply(simp_all add: fun_eq_iff nth_bit_of_add[simplified])
+   apply(auto)
+  by (meson dvd_imp_mod_0 even_add not_mod2_eq_Suc_0_eq_0)
+  
+
+lemma sequence_of_full_adders: 
+  assumes 
+    "s ''carry'' = 0" 
+    "\<forall>j \<le> k. s (operand_bit_to_var (CHR ''a'', j)) = nth_bit a j" 
+    "\<forall>j \<le> k. s (operand_bit_to_var (CHR ''b'', j)) = nth_bit b j"
+  shows
+   "t_small_step_fun (12 * (k + 1))
+                       (com_list_to_seq (map (\<lambda>i. full_adder i v) [0..<(k + 1)]), s)
+  = (SKIP, (\<lambda>w. (case var_to_var_bit w of
+    Some (w', m) \<Rightarrow> (if w' = v \<and> m \<le> k then nth_bit (a + b) m else s w) |
+    _ \<Rightarrow> (if w = ''carry'' then nth_carry k a b  
+          else s w))))"   
+  using assms
+proof(induction k)
+  case 0
+  then show ?case 
+      apply(auto simp: seq_terminates_iff)
+    apply(simp_all only: numeral_eq_Suc exists_terminating_iff)
+    apply auto
+    apply(rule t_small_step_fun_increase_time[where ?t=10 and ?t'=11])
+    apply auto
+    apply (subst full_adder_correct[where ?a=a and ?b=b])
+    by(auto simp: var_to_var_bit_eq_Some_iff numeral_eq_Suc split!: option.splits)
+next
+  case (Suc k)
+  hence "t_small_step_fun (24 + 12 * k)
+   (com_list_to_seq ((map (\<lambda>i. full_adder i v) [0..<(k + 1)]) @ [full_adder (k + 1) v]), s)
+    = (SKIP, (\<lambda>w. (case var_to_var_bit w of
+    Some (w', m) \<Rightarrow> (if w' = v \<and> m \<le> Suc k then nth_bit (a + b) m else s w) |
+    _ \<Rightarrow> (if w = ''carry'' then nth_carry (Suc k) a b  
+          else s w))))"
+    apply -
+    apply(rule t_small_step_fun_com_list_to_seq_terminates[where ?t1.0="12 * (k + 1)" and ?t2.0=11])
+      apply(auto simp: seq_terminates_iff)
+      apply(auto simp only: numeral_eq_Suc exists_terminating_iff fun_eq_iff)
+     apply auto
+    apply(subst full_adder_correct)
+    apply(simp_all)
+      apply(auto simp add: fun_eq_iff var_to_var_bit_eq_Some_iff var_bit_to_var_eq_iff split!: option.splits)
+    by(auto simp: var_bit_to_var_def)
+  thus ?case by auto
+qed 
+
+definition check_bit_non_zero:: "nat \<Rightarrow> vname \<Rightarrow> IMP_Minus_Minus_com" where
+"check_bit_non_zero i v = (IF (var_bit_to_var (v, i))\<noteq>0 THEN (''?$'' @ v) ::= A (N 1) ELSE SKIP)" 
+
+lemma result_of_check_bit_non_zero_sequence: 
+  "t_small_step_fun (4 * k)
+  (com_list_to_seq (map (\<lambda>i. check_bit_non_zero i v) [0..<k]), s)
+    = (SKIP, if (\<exists>j < k. s (var_bit_to_var (v, j)) \<noteq> 0) then (s(''?$'' @ v := 1)) else s)" 
+proof(induction k)
+  case 0
+  then show ?case by (auto simp: check_bit_non_zero_def t_small_step_fun_terminate_iff)
+next
+  case (Suc k)
+  hence "t_small_step_fun (4 * (Suc k))
+   (com_list_to_seq ((map (\<lambda>i. check_bit_non_zero i v) [0..<k]) 
+    @ [check_bit_non_zero k v]), s)
+    = (SKIP, if (\<exists>j < Suc k. s (var_bit_to_var (v, j)) \<noteq> 0) then (s(''?$'' @ v := 1)) else s)"
+     apply -
+    apply(rule t_small_step_fun_com_list_to_seq_terminates[where ?t1.0="4 * k" and ?t2.0=3])
+      apply(auto simp: seq_terminates_iff)
+      apply(auto simp only: numeral_eq_Suc exists_terminating_iff fun_eq_iff)
+    by (auto simp: check_bit_non_zero_def t_small_step_fun_terminate_iff less_Suc_eq split: if_splits)
+  thus ?case by simp
+qed
+
+definition binary_adder:: "nat \<Rightarrow> vname \<Rightarrow> vname \<Rightarrow> vname \<Rightarrow> IMP_Minus_Minus_com" where
+"binary_adder n v a b = 
+  copy_var_to_operand n (CHR ''a'') a ;;
+  (copy_var_to_operand n (CHR ''b'') b ;;
+  (com_list_to_seq (map (\<lambda>i. full_adder i v) [0..<n]) ;; 
+  ((''?$'' @ v) ::= A (N 0) ;;
+  (com_list_to_seq (map (\<lambda>i. check_bit_non_zero i v) [0..<n]) ;;
+  (copy_const_to_operand n (CHR ''a'') 0 ;;
+  copy_const_to_operand n (CHR ''b'') 0)))))"
+
+lemma binary_adder_correct: 
+  assumes "n > 0" "s ''carry'' = 0" 
+    "\<forall>j < n. s (operand_bit_to_var (CHR ''a'', j)) = 0"
+    "\<forall>j < n. s (operand_bit_to_var (CHR ''b'', j)) = 0"
+    "\<forall>j < n. s (var_bit_to_var (va, j)) = nth_bit a j" 
+    "\<forall>j < n. s (var_bit_to_var (vb, j)) = nth_bit b j"
+    "a + b < 2 ^ n" 
+  shows "t_small_step_fun (50 * (n + 1)) (binary_adder n v va vb, s) 
+    = (SKIP, (\<lambda>w. (case var_to_var_bit w of
+      Some (w', m) \<Rightarrow> (if w' = v \<and> m < n then nth_bit (a + b) m else s w) |
+      _ \<Rightarrow> (if w = ''carry'' then 0  
+            else if w = ''?$'' @ v then (if a + b \<noteq> 0 then 1 else 0) 
+            else s w))))"
+proof -
+  obtain k where k_def: "Suc k = n" using assms(1) gr0_implies_Suc by blast
+  hence "nth_carry k a b = 0" using assms no_overflow_condition by (metis diff_Suc_1)
+  thus ?thesis apply(simp only: binary_adder_def) 
+    apply(rule seq_terminates_when[where ?t1.0="2 * n" and ?t2.0="48 * n + 49"])
+     apply(auto)[1]
+     apply(auto simp: copy_var_to_operand_result)[1]
+    apply(rule seq_terminates_when[where ?t1.0="2 * n" and ?t2.0="46 * n + 48"])
+      apply auto[1]
+     apply(auto simp: copy_var_to_operand_result)[1]
+    apply(rule seq_terminates_when[where ?t1.0="12 * (k + 1)" and ?t2.0="34 * n + 47"])
+    using k_def apply auto[1]
+    using k_def[symmetric] apply simp
+     apply(rule sequence_of_full_adders[simplified])
+    using assms apply(simp split: option.splits)
+    using assms apply(auto split: option.splits)[1]
+    using assms apply(auto split: option.splits)[1]
+    apply(rule seq_terminates_when[where ?t1.0="1" and ?t2.0="34 * n + 45"])
+      apply auto[1]
+     apply auto[1]
+    apply(rule seq_terminates_when[where ?t1.0="4 * n" and ?t2.0="30 * n + 44"])
+      apply auto[1]
+     apply(auto simp: result_of_check_bit_non_zero_sequence)[1]
+    apply(rule seq_terminates_when[where ?t1.0="2 * n" and ?t2.0="28 * n + 43"])
+     apply(auto)[1]
+     apply(auto simp: copy_const_to_operand_result)[1]
+    apply(rule t_small_step_fun_increase_time[where ?t="2*n" and ?t' = "28 * n + 43"]) 
+     apply auto[1]
+    apply(simp only: copy_const_to_operand_result)
+    apply(auto simp only: fun_eq_iff split!: option.splits)
+       apply (simp_all add: var_to_var_bit_eq_Some_iff var_to_operand_bit_eq_Some_iff)
+    using k_def assms(2) assms(3) assms(4) assms(7) apply auto
+    by(frule all_bits_in_sum_zero_then, simp)+
+qed
+
+definition binary_adder_constant:: "nat \<Rightarrow> vname \<Rightarrow> vname \<Rightarrow> nat \<Rightarrow> IMP_Minus_Minus_com" where
+"binary_adder_constant n v a b = 
+  copy_var_to_operand n (CHR ''a'') a ;;
+  (copy_const_to_operand n (CHR ''b'') b ;;
+  (com_list_to_seq (map (\<lambda>i. full_adder i v) [0..<n]) ;; 
+  ((''?$'' @ v) ::= A (N 0) ;;
+  (com_list_to_seq (map (\<lambda>i. check_bit_non_zero i v) [0..<n]) ;;
+  (copy_const_to_operand n (CHR ''a'') 0 ;;
+  copy_const_to_operand n (CHR ''b'') 0)))))"
+
+lemma binary_adder_constant_correct: 
+  assumes "n > 0" "s ''carry'' = 0" 
+    "\<forall>j < n. s (operand_bit_to_var (CHR ''a'', j)) = 0"
+    "\<forall>j < n. s (operand_bit_to_var (CHR ''b'', j)) = 0"
+    "\<forall>j < n. s (var_bit_to_var (va, j)) = nth_bit a j" 
+    "a + b < 2 ^ n" 
+  shows "t_small_step_fun (50 * (n + 1)) (binary_adder_constant n v va b, s) 
+    = (SKIP, (\<lambda>w. (case var_to_var_bit w of
+      Some (w', m) \<Rightarrow> (if w' = v \<and> m < n then nth_bit (a + b) m else s w) |
+      _ \<Rightarrow> (if w = ''carry'' then 0  
+            else if w = ''?$'' @ v then (if a + b \<noteq> 0 then 1 else 0) 
+            else s w))))"
+proof -
+  obtain k where k_def: "Suc k = n" using assms(1) gr0_implies_Suc by blast
+  hence "nth_carry k a b = 0" using assms no_overflow_condition by (metis diff_Suc_1)
+  thus ?thesis apply(simp only: binary_adder_constant_def) 
+    apply(rule seq_terminates_when[where ?t1.0="2 * n" and ?t2.0="48 * n + 49"])
+     apply(auto)[1]
+     apply(auto simp: copy_var_to_operand_result)[1]
+    apply(rule seq_terminates_when[where ?t1.0="2 * n" and ?t2.0="46 * n + 48"])
+      apply auto[1]
+     apply(auto simp: copy_const_to_operand_result)[1]
+    apply(rule seq_terminates_when[where ?t1.0="12 * (k + 1)" and ?t2.0="34 * n + 47"])
+    using k_def apply auto[1]
+    using k_def[symmetric] apply simp
+     apply(rule sequence_of_full_adders[simplified])
+    using assms apply(simp split: option.splits)
+    using assms apply(auto split: option.splits)[1]
+    using assms apply(auto split: option.splits)[1]
+    apply(rule seq_terminates_when[where ?t1.0="1" and ?t2.0="34 * n + 45"])
+      apply auto[1]
+     apply auto[1]
+    apply(rule seq_terminates_when[where ?t1.0="4 * n" and ?t2.0="30 * n + 44"])
+      apply auto[1]
+     apply(auto simp: result_of_check_bit_non_zero_sequence)[1]
+    apply(rule seq_terminates_when[where ?t1.0="2 * n" and ?t2.0="28 * n + 43"])
+     apply(auto)[1]
+     apply(auto simp: copy_const_to_operand_result)[1]
+    apply(rule t_small_step_fun_increase_time[where ?t="2*n" and ?t' = "28 * n + 43"]) 
+     apply auto[1]
+    apply(simp only: copy_const_to_operand_result)
+    apply(auto simp only: fun_eq_iff split!: option.splits)
+       apply (simp_all add: var_to_var_bit_eq_Some_iff var_to_operand_bit_eq_Some_iff)
+    using k_def assms(2) assms(3) assms(4) assms(6) apply auto
+    by(frule all_bits_in_sum_zero_then, simp)+
+qed
+
+definition assign_var_carry_sub:: 
+  "nat \<Rightarrow> vname \<Rightarrow> nat \<Rightarrow> nat \<Rightarrow> nat \<Rightarrow> IMP_Minus_Minus_com" where
+"assign_var_carry_sub i v a b c = 
+  (var_bit_to_var (v, i)) ::= A (N (if b + c = 0 \<or> b + c = 2 then a 
+    else (if b + c = 1 \<and> a = 0 then 1 else 0))) ;; 
+  ''carry'' ::= A (N (if a < b + c then 1 else 0))"
+
+lemma result_of_assign_var_carry_sub:  
+  "t_small_step_fun 7 (assign_var_carry_sub i v a b c, s)
+    = (SKIP, s(var_bit_to_var (v, i) := (if b + c = 0 \<or> b + c = 2 then a 
+    else (if b + c = 1 \<and> a = 0 then 1 else 0)),
+     ''carry'' :=  (if a < b + c then 1 else 0)))"
+  by(auto simp: assign_var_carry_sub_def t_small_step_fun_terminate_iff)
+
+definition full_subtractor:: "nat \<Rightarrow> vname \<Rightarrow> IMP_Minus_Minus_com" where
+"full_subtractor i v  = (let assign = assign_var_carry_sub i v; op_a = operand_bit_to_var (CHR ''a'', i);
+  op_b = operand_bit_to_var (CHR ''b'', i) in 
+  IF op_a\<noteq>0 THEN 
+    IF ''carry''\<noteq>0 THEN
+      IF op_b\<noteq>0 THEN assign 1 1 1 
+      ELSE assign 1 1 0
+    ELSE 
+      IF op_b\<noteq>0 THEN assign 1 0 1
+      ELSE assign 1 0 0
+  ELSE 
+    IF ''carry''\<noteq>0 THEN
+      IF op_b\<noteq>0 THEN assign 0 1 1
+      ELSE assign 0 1 0
+    ELSE 
+      IF op_b\<noteq>0 THEN assign 0 0 1
+      ELSE assign 0 0 0)"
+
+lemma full_subtractor_correct_no_underflow: 
+  assumes "a \<ge> b"
+    "i = 0 \<longrightarrow> s ''carry'' = 0" 
+    "i > 0 \<longrightarrow> s ''carry'' = nth_carry_sub (i - 1) a b"
+    "s (operand_bit_to_var (CHR ''a'', i)) = nth_bit a i" 
+    "s (operand_bit_to_var (CHR ''b'', i)) = nth_bit b i"
+  shows "t_small_step_fun 10 (full_subtractor i v, s) = (SKIP, 
+    s(var_bit_to_var (v, i) := nth_bit (a - b) i, ''carry'' := nth_carry_sub i a b))" 
+  using assms 
+  apply(simp add: full_subtractor_def Let_def t_small_step_fun_terminate_iff result_of_assign_var_carry_sub)
+  apply(cases i)
+  apply(simp_all add: fun_eq_iff nth_bit_of_sub_n_no_underflow[simplified] Let_def)
+   apply(auto simp: mod2_eq_if)
+  by(frule nth_bit_eq_zero_or_one[where ?x="b div 2"], simp)+
+  
+
+lemma sequence_of_full_subtractors_no_underflow: 
+  assumes "a \<ge> b"
+    "s ''carry'' = 0" 
+    "\<forall>j \<le> k. s (operand_bit_to_var (CHR ''a'', j)) = nth_bit a j" 
+    "\<forall>j \<le> k. s (operand_bit_to_var (CHR ''b'', j)) = nth_bit b j"
+  shows
+   "t_small_step_fun (12 * (k + 1))
+                       (com_list_to_seq (map (\<lambda>i. full_subtractor i v) [0..<(k + 1)]), s)
+  = (SKIP, (\<lambda>w. (case var_to_var_bit w of
+    Some (w', m) \<Rightarrow> (if w' = v \<and> m \<le> k then nth_bit (a - b) m else s w) |
+    _ \<Rightarrow> (if w = ''carry'' then nth_carry_sub k a b  
+          else s w))))"   
+  sorry
+
+lemma sequence_of_full_subtractors_with_underflow: 
+  assumes "a < b"
+    "a < 2^(k + 2)" "b < 2^(k+2)" 
+    "s ''carry'' = 0" 
+    "\<forall>j \<le> k. s (operand_bit_to_var (CHR ''a'', j)) = nth_bit a j" 
+    "\<forall>j \<le> k. s (operand_bit_to_var (CHR ''b'', j)) = nth_bit b j"
+  shows
+   "t_small_step_fun (12 * (k + 1))
+                       (com_list_to_seq (map (\<lambda>i. full_subtractor i v) [0..<(k + 1)]), s)
+  = (SKIP, (\<lambda>w. (case var_to_var_bit w of
+    Some (w', m) \<Rightarrow> (if w' = v \<and> m \<le> k then nth_bit (2^(k+2) + a - b) m else s w) |
+    _ \<Rightarrow> (if w = ''carry'' then 1
+          else s w))))"   
+  sorry
+
+definition underflow_handler:: "nat \<Rightarrow> vname \<Rightarrow> IMP_Minus_Minus_com" where
+"underflow_handler n v = (IF ''carry''\<noteq>0 THEN (''carry'' ::= A (N 0) ;;
+  binary_assign_constant n v 0)
+  ELSE SKIP)" 
+
+definition binary_subtractor:: "nat \<Rightarrow> vname \<Rightarrow> vname \<Rightarrow> vname \<Rightarrow> IMP_Minus_Minus_com" where
+"binary_subtractor n v a b = 
+  copy_var_to_operand n (CHR ''a'') a ;;
+  (copy_var_to_operand n (CHR ''b'') b ;;
+  (com_list_to_seq (map (\<lambda>i. full_subtractor i v) [0..<n]) ;; 
+  underflow_handler n v ;;
+  ((''?$'' @ v) ::= A (N 0) ;;
+  (com_list_to_seq (map (\<lambda>i. check_bit_non_zero i v) [0..<n]) ;;
+  (copy_const_to_operand n (CHR ''a'') 0 ;;
+  copy_const_to_operand n (CHR ''b'') 0)))))"
+
+lemma binary_subtractor_correct: 
+  assumes "n > 0" "s ''carry'' = 0" 
+    "\<forall>j < n. s (operand_bit_to_var (CHR ''a'', j)) = 0"
+    "\<forall>j < n. s (operand_bit_to_var (CHR ''b'', j)) = 0"
+    "\<forall>j < n. s (var_bit_to_var (va, j)) = nth_bit a j" 
+    "\<forall>j < n. s (var_bit_to_var (vb, j)) = nth_bit b j"
+    "a + b < 2 ^ n" 
+  shows "t_small_step_fun (50 * (n + 1)) (binary_subtractor n v va vb, s) 
+    = (SKIP, (\<lambda>w. (case var_to_var_bit w of
+      Some (w', m) \<Rightarrow> (if w' = v \<and> m < n then nth_bit (a - b) m else s w) |
+      _ \<Rightarrow> (if w = ''carry'' then 0  
+            else if w = ''?$'' @ v then (if a - b \<noteq> 0 then 1 else 0) 
+            else s w))))"
+  sorry
+
+definition binary_subtractor_constant:: "nat \<Rightarrow> vname \<Rightarrow> vname \<Rightarrow> nat \<Rightarrow> IMP_Minus_Minus_com" where
+"binary_subtractor_constant n v a b = 
+  copy_var_to_operand n (CHR ''a'') a ;;
+  (copy_const_to_operand n (CHR ''b'') b ;;
+  (com_list_to_seq (map (\<lambda>i. full_adder i v) [0..<n]) ;; 
+  (underflow_handler n v ;;
+  ((''?$'' @ v) ::= A (N 0) ;;
+  (com_list_to_seq (map (\<lambda>i. check_bit_non_zero i v) [0..<n]) ;;
+  (copy_const_to_operand n (CHR ''a'') 0 ;;
+  copy_const_to_operand n (CHR ''b'') 0))))))"
+
+lemma binary_subtractor_constant_correct: 
+ assumes "n > 0" "s ''carry'' = 0" 
+    "\<forall>j < n. s (operand_bit_to_var (CHR ''a'', j)) = 0"
+    "\<forall>j < n. s (operand_bit_to_var (CHR ''b'', j)) = 0"
+    "\<forall>j < n. s (var_bit_to_var (va, j)) = nth_bit a j" 
+    "a + b < 2 ^ n" 
+  shows "t_small_step_fun (50 * (n + 1)) (binary_subtractor_constant n v va b, s) 
+    = (SKIP, (\<lambda>w. (case var_to_var_bit w of
+      Some (w', m) \<Rightarrow> (if w' = v \<and> m < n then nth_bit (a - b) m else s w) |
+      _ \<Rightarrow> (if w = ''carry'' then 0  
+            else if w = ''?$'' @ v then (if a - b \<noteq> 0 then 1 else 0) 
+            else s w))))"
+  sorry
+
+definition binary_subtractor_constant':: "nat \<Rightarrow> vname \<Rightarrow> nat \<Rightarrow> vname \<Rightarrow> IMP_Minus_Minus_com" where
+"binary_subtractor_constant' n v a b = 
+  copy_const_to_operand n (CHR ''a'') a ;;
+  (copy_var_to_operand n (CHR ''b'') b ;;
+  (com_list_to_seq (map (\<lambda>i. full_adder i v) [0..<n]) ;; 
+  (underflow_handler n v ;;
+  ((''?$'' @ v) ::= A (N 0) ;;
+  (com_list_to_seq (map (\<lambda>i. check_bit_non_zero i v) [0..<n]) ;;
+  (copy_const_to_operand n (CHR ''a'') 0 ;;
+  copy_const_to_operand n (CHR ''b'') 0))))))"
+
+lemma binary_subtractor_constant_correct': 
+ assumes "n > 0" "s ''carry'' = 0" 
+    "\<forall>j < n. s (operand_bit_to_var (CHR ''a'', j)) = 0"
+    "\<forall>j < n. s (operand_bit_to_var (CHR ''b'', j)) = 0"
+    "\<forall>j < n. s (var_bit_to_var (vb, j)) = nth_bit b j" 
+    "a + b < 2 ^ n" 
+  shows "t_small_step_fun (50 * (n + 1)) (binary_subtractor_constant' n v a vb, s) 
+    = (SKIP, (\<lambda>w. (case var_to_var_bit w of
+      Some (w', m) \<Rightarrow> (if w' = v \<and> m < n then nth_bit (a - b) m else s w) |
+      _ \<Rightarrow> (if w = ''carry'' then 0  
+            else if w = ''?$'' @ v then (if a - b \<noteq> 0 then 1 else 0) 
+            else s w))))"
+  sorry
+
+
+end
